LL1 Parser: add JSON lexer

thys/LL1_Parser/Json_Parser.thy
@@ -1,12 +1,11 @@
 subsection \<open>Generating a JSON Parser\<close>
 
 theory Json_Parser
-  imports LL1_Parser_show "Show.Show_Instances"
+  imports LL1_Parser_show "Show.Show_Instances" "HOL-Library.Code_Target_Numeral"
 begin
 
 datatype terminal =
-    TInt
-  | Float
+    TNum
   | Str
   | Tru
   | Fls
@@ -35,8 +34,7 @@ definition jsonGrammar :: "(nterminal, terminal) grammar" where
     (Value, [T LeftBrace, NT Pairs, T RightBrace]),
     (Value, [T LeftBrack, NT Elts, T RightBrack]),
     (Value, [T Str]),
-    (Value, [T TInt]),
-    (Value, [T Float]),
+    (Value, [T TNum]),
     (Value, [T Tru]),
     (Value, [T Fls]),
     (Value, [T Null]),
@@ -59,12 +57,23 @@ definition jsonGrammar :: "(nterminal, terminal) grammar" where
 definition pt :: "(nterminal, terminal) ll1_parse_table" where
   "pt = mkParseTable jsonGrammar"
 
+datatype json_number =
+  JsonNumber
+    (neg: bool)
+    (int:  nat)
+    (frac: "string option") \<comment> \<open>string due to leading zeros\<close>
+    (exp_neg: bool)
+    (exp: "nat option")
+
+hide_const (open)
+  json_number.neg json_number.int json_number.frac json_number.exp_neg json_number.exp
+
 datatype lex =
-    LInt (lex_int: int)
-  | LFloat
+    LNum (lex_num: json_number)
   | LStr (lex_str: string)
   | LNone
 
+derive "show" "json_number"
 derive "show" "lex"
 
 definition
@@ -98,7 +107,7 @@ abbreviation
   "TruS \<equiv> mkS Tru"
 
 definition
-  "IntS s = (TInt, LInt s)"
+  "IntS n = (TNum, LNum (JsonNumber False n None False None))"
 
 text\<open>Example input:
 \<^verbatim>\<open>{
@@ -185,9 +194,7 @@ datatype JSON =
   Object "(string \<times> JSON) list"
 | Array "JSON list"
 | String string \<comment>\<open>An Isabelle string rather than a JSON string\<close>
-| Int int \<comment>\<open>The number type is split into natural Isabelle/HOL types\<close>
-| Nat nat
-| Rat nat int
+| Num json_number
 | Boolean bool \<comment>\<open>True and False are contracted to one constructor\<close>
 | Nil
 
@@ -199,8 +206,7 @@ where
 definition
   "json_leaf \<equiv> \<lambda>(t, s). (case t of
     Str => JSON.String (lex_str s) |
-    TInt => JSON.Int (lex_int s) |
-    Float \<Rightarrow> JSON.Rat 1 0 |
+    TNum => JSON.Num (lex_num s) |
     Tru \<Rightarrow> JSON.Boolean True |
     Fls => JSON.Boolean False |
     Null => JSON.Nil |
@@ -274,9 +280,12 @@ lemma "parse_tree_to_json (the_RESULT (parse pt (NT (start jsonGrammar))
     [(''items'',
       Array
        [Object
-         [(''id'', JSON.Int 65), (''description'', String ''Title''),
+         [(''id'', JSON.Num (JsonNumber False 65 None False None)),
+          (''description'', String ''Title''),
           (''visible'', Boolean False)],
-        Object [(''id'', JSON.Int 42), (''visible'', Boolean True)]])]"
+        Object
+          [(''id'', JSON.Num (JsonNumber False 42 None False None)),
+           (''visible'', Boolean True)]])]"
   by eval
 
 text \<open>
@@ -285,5 +294,858 @@ to the production rules.
 While this would be possible in Isabelle/HOL, it would give little advantage over defining
 the reader function directly, since we are missing dependent types.
 \<close>
+
+subsection \<open>JSON Lexing as LL1 Parsing\<close>
+
+definition
+  "is_digit x \<equiv> x \<in> {
+    CHR ''0'', CHR ''1'', CHR ''2'', CHR ''3'', CHR ''4'', CHR ''5'', CHR ''6'', CHR ''7'',
+    CHR ''8'', CHR ''9''}"
+
+definition is_hex :: "char \<Rightarrow> bool" where
+  "is_hex c \<equiv>
+   let n = of_char c :: nat in
+     is_digit c \<or>
+     (of_char (CHR ''A'') \<le> n \<and> n \<le> of_char (CHR ''F'')) \<or>
+     (of_char (CHR ''a'') \<le> n \<and> n \<le> of_char (CHR ''f''))"
+
+datatype chr =
+    COneNine | CZero
+  | CMinus | CPlus | CDot | CE | Ce
+  | CSpace | CWS
+  | CQuote | CBackslash | CSlash
+  | Ct | Cr | Cu
+  | Cf | Ca | Cl | Cs
+  | Cn | Cb
+  | CLBrace | CRBrace | CLBrack | CRBrack
+  | CColon | CComma
+  | CStringChar | CControlChar
+  | CHex
+
+datatype lterminal = LRoot | LStartStr | LEscape
+  | LStartInt | LZero | LMinus | LStartFrac | LFrac | LExp | LStartExp | LExpSign
+  | LUnicode1 | LUnicode2 | LUnicode3 | LUnicode4
+
+definition jsonLex :: "(lterminal + terminal, chr) grammar" where
+  "jsonLex = G (Inl LRoot) [
+
+  \<comment>\<open> whitespace \<close>
+  (Inl LRoot, []),
+  (Inl LRoot, [T CWS, NT (Inl LRoot)]),
+  (Inl LRoot, [T CSpace, NT (Inl LRoot)]),
+
+  \<comment>\<open> punctuation \<close>
+  (Inl LRoot, [T CLBrace, NT (Inr LeftBrace), NT (Inl LRoot)]),
+  (Inl LRoot, [T CRBrace, NT (Inr RightBrace), NT (Inl LRoot)]),
+  (Inl LRoot, [T CLBrack, NT (Inr LeftBrack), NT (Inl LRoot)]),
+  (Inl LRoot, [T CRBrack, NT (Inr RightBrack), NT (Inl LRoot)]),
+  (Inl LRoot, [T CColon,  NT (Inr Colon), NT (Inl LRoot)]),
+  (Inl LRoot, [T CComma,  NT (Inr Comma), NT (Inl LRoot)]),
+  (Inr LeftBrace, []),
+  (Inr RightBrace, []),
+  (Inr LeftBrack, []),
+  (Inr RightBrack, []),
+  (Inr Colon, []),
+  (Inr Comma, []),
+
+  \<comment>\<open> true  \<close>
+  (Inl LRoot, [T Ct, T Cr, T Cu, T Ce, NT (Inr Tru), NT (Inl LRoot)]),
+  (Inr Tru, []),
+
+  \<comment>\<open> false \<close>
+  (Inl LRoot, [T Cf, T Ca, T Cl, T Cs, T Ce, NT (Inr Fls), NT (Inl LRoot)]),
+  (Inr Fls, []),
+
+  \<comment>\<open> null \<close>
+  (Inl LRoot, [T Cn, T Cu, T Cl, T Cl, NT (Inr Null), NT (Inl LRoot)]),
+  (Inr Null, []),
+
+  \<comment>\<open> ---------- string ---------- \<close>
+  (Inl LRoot, [T CQuote, NT (Inl LStartStr), NT (Inl LRoot)]),
+
+  \<comment>\<open> unescaped characters allowed inside strings \<close>
+  (Inl LStartStr,   [T CStringChar,  NT (Inr Str)]),
+  (Inl LStartStr,   [T CHex,         NT (Inr Str)]),
+  (Inl LStartStr,   [T CZero,        NT (Inr Str)]),
+  (Inl LStartStr,   [T COneNine,     NT (Inr Str)]),
+  (Inl LStartStr,   [T CMinus,       NT (Inr Str)]),
+  (Inl LStartStr,   [T CPlus,        NT (Inr Str)]),
+  (Inl LStartStr,   [T CDot,         NT (Inr Str)]),
+  (Inl LStartStr,   [T CE,           NT (Inr Str)]),
+  (Inl LStartStr,   [T Ce,           NT (Inr Str)]),
+  (Inl LStartStr,   [T CSlash,       NT (Inr Str)]),
+  
+  (Inl LStartStr,   [T Ct, NT (Inr Str)]),
+  (Inl LStartStr,   [T Cr, NT (Inr Str)]),
+  (Inl LStartStr,   [T Cu, NT (Inr Str)]),
+  (Inl LStartStr,   [T Cf, NT (Inr Str)]),
+  (Inl LStartStr,   [T Ca, NT (Inr Str)]),
+  (Inl LStartStr,   [T Cl, NT (Inr Str)]),
+  (Inl LStartStr,   [T Cs, NT (Inr Str)]),
+  (Inl LStartStr,   [T Cn, NT (Inr Str)]),
+  (Inl LStartStr,   [T Cb, NT (Inr Str)]),
+  
+  (Inl LStartStr,   [T CLBrace,  NT (Inr Str)]),
+  (Inl LStartStr,   [T CRBrace,  NT (Inr Str)]),
+  (Inl LStartStr,   [T CLBrack,  NT (Inr Str)]),
+  (Inl LStartStr,   [T CRBrack,  NT (Inr Str)]),
+  (Inl LStartStr,   [T CColon,   NT (Inr Str)]),
+  (Inl LStartStr,   [T CComma,   NT (Inr Str)]),
+  (Inl LStartStr,   [T CSpace,      NT (Inr Str)]),
+  
+  (Inr Str,   [T CStringChar,  NT (Inr Str)]),
+  (Inr Str,   [T CHex,         NT (Inr Str)]),
+  (Inr Str,   [T CZero,        NT (Inr Str)]),
+  (Inr Str,   [T COneNine,     NT (Inr Str)]),
+  (Inr Str,   [T CMinus,       NT (Inr Str)]),
+  (Inr Str,   [T CPlus,        NT (Inr Str)]),
+  (Inr Str,   [T CDot,         NT (Inr Str)]),
+  (Inr Str,   [T CE,           NT (Inr Str)]),
+  (Inr Str,   [T Ce,           NT (Inr Str)]),
+  (Inr Str,   [T CSlash,       NT (Inr Str)]),
+  
+  (Inr Str,   [T Ct, NT (Inr Str)]),
+  (Inr Str,   [T Cr, NT (Inr Str)]),
+  (Inr Str,   [T Cu, NT (Inr Str)]),
+  (Inr Str,   [T Cf, NT (Inr Str)]),
+  (Inr Str,   [T Ca, NT (Inr Str)]),
+  (Inr Str,   [T Cl, NT (Inr Str)]),
+  (Inr Str,   [T Cs, NT (Inr Str)]),
+  (Inr Str,   [T Cn, NT (Inr Str)]),
+  (Inr Str,   [T Cb, NT (Inr Str)]),
+  
+  (Inr Str,   [T CLBrace,  NT (Inr Str)]),
+  (Inr Str,   [T CRBrace,  NT (Inr Str)]),
+  (Inr Str,   [T CLBrack,  NT (Inr Str)]),
+  (Inr Str,   [T CRBrack,  NT (Inr Str)]),
+  (Inr Str,   [T CColon,   NT (Inr Str)]),
+  (Inr Str,   [T CComma,   NT (Inr Str)]),
+  (Inr Str,   [T CSpace,      NT (Inr Str)]),
+  
+  \<comment>\<open> escape sequence introducer \<close>
+  (Inr Str,       [T CBackslash, NT (Inl LEscape), NT (Inr Str)]),
+  (Inl LStartStr, [T CBackslash, NT (Inl LEscape), NT (Inr Str)]),
+  (Inl LEscape,   [T CQuote]),
+  (Inl LEscape,   [T CBackslash]),
+  (Inl LEscape,   [T CSlash]),
+  (Inl LEscape,   [T Cb]),
+  (Inl LEscape,   [T Cf]),
+  (Inl LEscape,   [T Cn]),
+  (Inl LEscape,   [T Cr]),
+  (Inl LEscape,   [T Ct]),
+
+  \<comment>\<open> unicode code points \<close>
+  (Inl LEscape,   [T Cu, NT (Inl LUnicode1)]),
+
+  (Inl LUnicode1, [T CZero,    NT (Inl LUnicode2)]),
+  (Inl LUnicode1, [T COneNine, NT (Inl LUnicode2)]),
+  (Inl LUnicode1, [T CHex,     NT (Inl LUnicode2)]),
+  (Inl LUnicode1, [T Ca,       NT (Inl LUnicode2)]),
+  (Inl LUnicode1, [T Cb,       NT (Inl LUnicode2)]),
+  (Inl LUnicode1, [T Ce,       NT (Inl LUnicode2)]),
+  (Inl LUnicode1, [T CE,       NT (Inl LUnicode2)]),
+  (Inl LUnicode1, [T Cf,       NT (Inl LUnicode2)]),
+
+  (Inl LUnicode2, [T CZero,    NT (Inl LUnicode3)]),
+  (Inl LUnicode2, [T COneNine, NT (Inl LUnicode3)]),
+  (Inl LUnicode2, [T CHex,     NT (Inl LUnicode3)]),
+  (Inl LUnicode2, [T Ca,       NT (Inl LUnicode3)]),
+  (Inl LUnicode2, [T Cb,       NT (Inl LUnicode3)]),
+  (Inl LUnicode2, [T Ce,       NT (Inl LUnicode3)]),
+  (Inl LUnicode2, [T CE,       NT (Inl LUnicode3)]),
+  (Inl LUnicode2, [T Cf,       NT (Inl LUnicode3)]),
+
+  (Inl LUnicode3, [T CZero,    NT (Inl LUnicode4)]),
+  (Inl LUnicode3, [T COneNine, NT (Inl LUnicode4)]),
+  (Inl LUnicode3, [T CHex,     NT (Inl LUnicode4)]),
+  (Inl LUnicode3, [T Ca,       NT (Inl LUnicode4)]),
+  (Inl LUnicode3, [T Cb,       NT (Inl LUnicode4)]),
+  (Inl LUnicode3, [T Ce,       NT (Inl LUnicode4)]),
+  (Inl LUnicode3, [T CE,       NT (Inl LUnicode4)]),
+  (Inl LUnicode3, [T Cf,       NT (Inl LUnicode4)]),
+
+  (Inl LUnicode4, [T CZero]),
+  (Inl LUnicode4, [T COneNine]),
+  (Inl LUnicode4, [T CHex]),
+  (Inl LUnicode4, [T Ca]),
+  (Inl LUnicode4, [T Cb]),
+  (Inl LUnicode4, [T Ce]),
+  (Inl LUnicode4, [T CE]),
+  (Inl LUnicode4, [T Cf]),
+
+  \<comment>\<open> closing quote \<close>
+  (Inl LStartStr, [T CQuote]),
+  (Inr Str,       [T CQuote]),
+
+  \<comment>\<open> integer \<close>
+  (Inl LRoot, [T CZero, NT (Inl LZero)]),
+  (Inl LRoot, [T CMinus, NT (Inl LMinus)]),
+  (Inl LRoot, [T COneNine, NT (Inl LStartInt)]),
+
+  (Inl LMinus, [T CZero, NT (Inl LZero)]),
+  (Inl LMinus, [T COneNine, NT (Inl LStartInt)]),
+
+  (Inl LZero, [T CDot, NT (Inl LStartFrac)]),
+  (Inl LZero, [T CComma, NT (Inr Comma), NT (Inl LRoot)]),
+  (Inl LZero, [T CRBrack, NT (Inr RightBrack), NT (Inl LRoot)]),
+  (Inl LZero, [T CRBrace, NT (Inr RightBrace), NT (Inl LRoot)]),
+  (Inl LZero, [T CWS, NT (Inl LRoot)]),
+  (Inl LZero, [T CSpace, NT (Inl LRoot)]),
+  (Inl LZero, []),
+
+  (Inl LStartInt, [T CZero, NT (Inr TNum)]),
+  (Inl LStartInt, [T COneNine, NT (Inr TNum)]),
+  (Inl LStartInt, [T CDot, NT (Inl LStartFrac)]),
+  (Inl LStartInt, [T CComma, NT (Inr Comma), NT (Inl LRoot)]),
+  (Inl LStartInt, [T CRBrack, NT (Inr RightBrack), NT (Inl LRoot)]),
+  (Inl LStartInt, [T CRBrace, NT (Inr RightBrace), NT (Inl LRoot)]),
+  (Inl LStartInt, [T CWS, NT (Inl LRoot)]),
+  (Inl LStartInt, [T CSpace, NT (Inl LRoot)]),
+  (Inl LStartInt, []),
+
+  (Inr TNum, [T CZero, NT (Inr TNum)]),
+  (Inr TNum, [T COneNine, NT (Inr TNum)]),
+  (Inr TNum, [T CComma, NT (Inr Comma), NT (Inl LRoot)]),
+  (Inr TNum, [T CRBrack, NT (Inr RightBrack), NT (Inl LRoot)]),
+  (Inr TNum, [T CRBrace, NT (Inr RightBrace), NT (Inl LRoot)]),
+  (Inr TNum, [T CWS, NT (Inl LRoot)]),
+  (Inr TNum, [T CSpace, NT (Inl LRoot)]),
+  (Inr TNum, []),
+
+  \<comment>\<open> fraction \<close>
+  (Inr TNum, [T CDot, NT (Inl LStartFrac)]),
+
+  (Inl LStartFrac, [T CZero,    NT (Inl LFrac)]),
+  (Inl LStartFrac, [T COneNine, NT (Inl LFrac)]),
+
+  (Inl LFrac, [T CZero, NT (Inl LFrac)]),
+  (Inl LFrac, [T COneNine, NT (Inl LFrac)]),
+  (Inl LFrac, [T CComma, NT (Inr Comma), NT (Inl LRoot)]),
+  (Inl LFrac, [T CRBrack, NT (Inr RightBrack), NT (Inl LRoot)]),
+  (Inl LFrac, [T CRBrace, NT (Inr RightBrace), NT (Inl LRoot)]),
+  (Inl LFrac, [T CWS, NT (Inl LRoot)]),
+  (Inl LFrac, [T CSpace, NT (Inl LRoot)]),
+  (Inl LFrac, []),
+
+  \<comment>\<open> exponent \<close>
+  (Inl LZero,     [T CE, NT (Inl LStartExp)]),
+  (Inl LZero,     [T Ce, NT (Inl LStartExp)]),
+  (Inr TNum,      [T CE, NT (Inl LStartExp)]),
+  (Inr TNum,      [T Ce, NT (Inl LStartExp)]),
+  (Inl LStartInt, [T CE, NT (Inl LStartExp)]),
+  (Inl LStartInt, [T Ce, NT (Inl LStartExp)]),
+  (Inl LFrac,     [T CE, NT (Inl LStartExp)]),
+  (Inl LFrac,     [T Ce, NT (Inl LStartExp)]),
+
+  (Inl LStartExp, [T CPlus,    NT (Inl LExpSign)]),
+  (Inl LStartExp, [T CMinus,   NT (Inl LExpSign)]),
+  (Inl LStartExp, [T CZero,    NT (Inl LExp)]),
+  (Inl LStartExp, [T COneNine, NT (Inl LExp)]),
+
+  (Inl LExpSign, [T CZero,    NT (Inl LExp)]),
+  (Inl LExpSign, [T COneNine, NT (Inl LExp)]),
+
+  (Inl LExp, [T CZero,    NT (Inl LExp)]),
+  (Inl LExp, [T COneNine, NT (Inl LExp)]),
+  (Inl LExp, [T CComma,   NT (Inr Comma),      NT (Inl LRoot)]),
+  (Inl LExp, [T CRBrack,  NT (Inr RightBrack), NT (Inl LRoot)]),
+  (Inl LExp, [T CRBrace,  NT (Inr RightBrace), NT (Inl LRoot)]),
+  (Inl LExp, [T CWS,      NT (Inl LRoot)]),
+  (Inl LExp, [T CSpace,   NT (Inl LRoot)]),
+  (Inl LExp, [])
+]"
+
+definition lex_pt :: "(lterminal + terminal, chr) ll1_parse_table" where
+  "lex_pt = mkParseTable jsonLex"
+
+\<comment> \<open>The parse table is valid.\<close>
+lemma "case lex_pt of ERROR_GRAMMAR_NOT_LL1_AMB_LA _ \<Rightarrow> False | _ \<Rightarrow> True"
+  by eval
+
+definition is_ws :: "char \<Rightarrow> bool" where
+  "is_ws c \<equiv> c = CHR '' '' \<or> c = CHR ''\<newline>'' \<or> c = CHR 0x0D \<or> c = CHR 0x09"
+
+definition is_control :: "char \<Rightarrow> bool" where
+  "is_control c \<equiv> of_char c < (32::nat)"
+
+definition char_to_chr :: "char \<Rightarrow> chr" where
+  "char_to_chr c =
+    (if c = CHR ''{'' then CLBrace else
+     if c = CHR ''}'' then CRBrace else
+     if c = CHR ''['' then CLBrack else
+     if c = CHR '']'' then CRBrack else
+     if c = CHR '':'' then CColon else
+     if c = CHR '','' then CComma else
+
+     if c = CHR ''\"'' then CQuote else
+     if c = CHR 0x5C   then CBackslash else
+     if c = CHR ''/''  then CSlash else
+
+     if c = CHR ''0'' then CZero else
+     if is_digit c then COneNine else
+
+     if c = CHR ''-'' then CMinus else
+     if c = CHR ''+'' then CPlus else
+     if c = CHR ''.'' then CDot else
+     if c = CHR ''E'' then CE else
+     if c = CHR ''e'' then Ce else
+
+     if c = CHR ''t'' then Ct else
+     if c = CHR ''r'' then Cr else
+     if c = CHR ''u'' then Cu else
+     if c = CHR ''f'' then Cf else
+     if c = CHR ''a'' then Ca else
+     if c = CHR ''l'' then Cl else
+     if c = CHR ''s'' then Cs else
+     if c = CHR ''n'' then Cn else
+     if c = CHR ''b'' then Cb else
+
+     if c = CHR '' '' then CSpace else
+     if is_ws c then CWS else
+     if is_control c then CControlChar else
+     if is_hex c then CHex else
+     CStringChar)"
+
+definition
+  "mk_chrs = map (\<lambda>x. (char_to_chr x, x))"
+
+derive "show" "chr"
+
+definition lex_leaf ::
+  "(chr \<times> char) \<Rightarrow> (char + terminal \<times> lex) list" where
+  "lex_leaf = (\<lambda>(t, c). [Inl c])"
+
+definition string_to_nat :: "string \<Rightarrow> nat" where
+  "string_to_nat s = horner_sum (\<lambda>c. of_char c - of_char (CHR ''0'')) 10 (rev s)"
+
+definition
+  "is_1_9 c \<equiv> of_char (CHR ''0'') < (of_char c :: nat) \<and> (of_char c :: nat) \<le> of_char (CHR ''9'')"
+
+definition
+  "ends_int c \<equiv> c \<in> {CHR '','', CHR ''}'', CHR '']''} \<or> is_ws c"
+
+definition combine_strings where
+  "combine_strings xs \<equiv> let
+      ys = concat xs;
+      as = takeWhile (\<lambda>Inl c \<Rightarrow> \<not> ends_int c | Inr (Str, LStr s) \<Rightarrow> True | _ \<Rightarrow> False) ys;
+      s  = List.maps (\<lambda>Inl c \<Rightarrow> [c] | Inr (Str, LStr s) \<Rightarrow> s    | _ \<Rightarrow> '''') as;
+      bs = dropWhile (\<lambda>Inl c \<Rightarrow> \<not> ends_int c | Inr (Str, LStr s) \<Rightarrow> True | _ \<Rightarrow> False) ys
+  in (s, bs)"
+
+definition map_escape :: "char \<Rightarrow> char" where
+  "map_escape c \<equiv> case c of
+      CHR ''\"'' \<Rightarrow> CHR ''\"''
+    | CHR 0x5C   \<Rightarrow> CHR 0x5C
+    | CHR ''/''  \<Rightarrow> CHR ''/''
+    | CHR ''b''  \<Rightarrow> CHR 0x08
+    | CHR ''f''  \<Rightarrow> CHR 12
+    | CHR ''n''  \<Rightarrow> CHR ''\<newline>''
+    | CHR ''r''  \<Rightarrow> CHR 13
+    | CHR ''t''  \<Rightarrow> CHR 0x09
+    | _ \<Rightarrow> c"
+
+definition map_int where
+  "map_int c s \<equiv>
+  let
+    n  = string_to_nat s;
+    neg  = (c = CHR ''-'');
+    num = JsonNumber neg n None False None
+   in Inr (TNum, LNum num)"
+
+definition map_rat where
+  "map_rat c s \<equiv>
+  let
+    ns = takeWhile (\<lambda>c. c \<noteq> CHR ''.'') s;
+    fs = tl (dropWhile (\<lambda>c. c \<noteq> CHR ''.'') s);
+    n  = string_to_nat ns;
+    neg  = (c = CHR ''-'');
+    num = JsonNumber neg n (Some fs) False None
+   in Inr (TNum, LNum num)"
+
+definition map_rat_exp where
+  "map_rat_exp c s \<equiv>
+  let
+    coeff_s = takeWhile (\<lambda>c. c \<noteq> CHR ''e'' \<and> c \<noteq> CHR ''E'') s;
+    exp_s   = tl (dropWhile (\<lambda>c. c \<noteq> CHR ''e'' \<and> c \<noteq> CHR ''E'') s);
+    
+    exp_neg = (hd exp_s = CHR ''-'');
+    exp_val = string_to_nat (if hd exp_s = CHR ''-'' \<or> hd exp_s = CHR ''+'' 
+                             then tl exp_s else exp_s);
+
+    ns = takeWhile (\<lambda>c. c \<noteq> CHR ''.'') coeff_s;
+    fs = (let rem = dropWhile (\<lambda>c. c \<noteq> CHR ''.'') coeff_s in 
+          if rem = [] then [] else tl rem);
+    
+    n  = string_to_nat ns;
+    neg  = (c = CHR ''-'');
+    num = JsonNumber neg n (Some fs) exp_neg (Some exp_val)
+   in Inr (TNum, LNum num)"
+
+definition map_rat_int where
+  "map_rat_int c s \<equiv>
+  if CHR ''e'' \<in> set s \<or> CHR ''E'' \<in> set s then
+    map_rat_exp c s
+  else if CHR ''.'' \<in> set s then
+    map_rat c s
+  else
+    map_int c s"
+
+definition hex_val :: "char \<Rightarrow> nat" where
+  "hex_val c = (let n = of_char c :: nat in
+     (if of_char CHR ''0'' \<le> n \<and> n \<le> of_char CHR ''9'' then
+        n - of_char CHR ''0''
+      else if of_char CHR ''A'' \<le> n \<and> n \<le> of_char CHR ''F'' then
+        10 + n - of_char CHR ''A''
+      else 10 + n - of_char CHR ''a''))"
+
+definition hex4_to_nat :: "char list \<Rightarrow> nat" where
+  "hex4_to_nat cs = horner_sum hex_val 16 (rev cs)"
+
+definition utf8_encode_bmp :: "nat \<Rightarrow> string" where
+  "utf8_encode_bmp u =
+     (if u < 0x80 then
+        [char_of u]
+      else if u < 0x800 then
+        [ char_of (0xC0 + u div 64),
+          char_of (0x80 + u mod 64) ]
+      else
+        [ char_of (0xE0 + u div 4096),
+          char_of (0x80 + (u div 64) mod 64),
+          char_of (0x80 + u mod 64) ])"
+
+definition decode_unicode_escape :: "string \<Rightarrow> string" where
+  "decode_unicode_escape cs =
+     utf8_encode_bmp (hex4_to_nat cs)"
+
+definition lex_node ::
+  "(char + terminal \<times> lex) list list \<Rightarrow> lterminal + terminal \<Rightarrow> (char + terminal \<times> lex) list" where
+  "lex_node xs nt =
+    (case nt of
+       Inl LRoot \<Rightarrow> (case xs of
+        [Inl c] # _ \<Rightarrow>
+          if is_1_9 c \<or> c = CHR ''0'' \<or> c = CHR ''-'' then
+          let (s, bs) = combine_strings xs
+           in map_rat_int c s # bs
+          else
+            concat xs
+       | _ \<Rightarrow> concat xs
+       )
+     | Inl LZero \<Rightarrow> concat xs
+     | Inl LMinus \<Rightarrow> concat xs
+     | Inl LStartStr \<Rightarrow> (
+       let xs = (case xs of [Inl (CHR 0x5C)] # xs \<Rightarrow> xs | _ \<Rightarrow> xs);
+           ys = concat xs;
+           s  = List.maps (\<lambda>Inl c \<Rightarrow> [c]  | Inr (Str, LStr s) \<Rightarrow> s    | _ \<Rightarrow> '''') ys;
+           s  = butlast s
+        in [Inr (Str, LStr s)]
+      )
+     | Inl LStartInt \<Rightarrow>
+       let (s, bs) = combine_strings xs
+        in (Inr (Str, LStr s)) # bs 
+     | Inl LStartFrac \<Rightarrow>
+       let (s, bs) = combine_strings xs
+        in (Inr (Str, LStr s)) # bs 
+     | Inl LExp \<Rightarrow>
+       let (s, bs) = combine_strings xs
+        in (Inr (Str, LStr s)) # bs 
+     | Inl LExpSign \<Rightarrow>
+       let (s, bs) = combine_strings xs
+        in (Inr (Str, LStr s)) # bs 
+     | Inl LStartExp \<Rightarrow>
+       let (s, bs) = combine_strings xs
+        in (Inr (Str, LStr s)) # bs 
+     | Inr Tru \<Rightarrow> [Inr (Tru, LNone)]
+     | Inr Fls \<Rightarrow> [Inr (Fls, LNone)]
+     | Inr Null \<Rightarrow> [Inr (Null, LNone)]
+     | Inr Str \<Rightarrow>
+       let xs = (case xs of [Inl (CHR 0x5C)] # xs \<Rightarrow> xs | _ \<Rightarrow> xs);
+           ys = concat xs;
+           s  = List.maps (\<lambda>Inl c \<Rightarrow> [c]  | Inr (Str, LStr s) \<Rightarrow> s    | _ \<Rightarrow> '''') ys
+        in [Inr (Str, LStr s)]
+     | Inl LEscape \<Rightarrow> (case xs of
+         [[Inl c]] \<Rightarrow> [Inl (map_escape c)]
+       | _ \<Rightarrow> tl (concat xs) \<comment> \<open>for unicode code points\<close>
+       )
+     | Inr LeftBrack  \<Rightarrow> [Inr (LeftBrack, LNone)]
+     | Inr RightBrack \<Rightarrow> [Inr (RightBrack, LNone)]
+     | Inr LeftBrace  \<Rightarrow> [Inr (LeftBrace, LNone)]
+     | Inr RightBrace \<Rightarrow> [Inr (RightBrace, LNone)]
+     | Inr Comma      \<Rightarrow> [Inr (Comma, LNone)]
+     | Inr Colon      \<Rightarrow> [Inr (Colon, LNone)]
+     | Inr TNum \<Rightarrow>
+       let (s, bs) = combine_strings xs
+        in (Inr (Str, LStr s)) # bs
+     | Inl LFrac \<Rightarrow> concat xs
+     | Inl LUnicode1 \<Rightarrow>
+       let (s, _) = combine_strings xs;
+                s = decode_unicode_escape s
+        in [Inr (Str, LStr s)]
+     | Inl LUnicode2 \<Rightarrow> concat xs
+     | Inl LUnicode3 \<Rightarrow> concat xs
+     | Inl LUnicode4 \<Rightarrow> concat xs
+    )"
+
+definition
+  "lex_tree_to_lex_list xs = [sum.projr x . x \<leftarrow> fold_parse_tree lex_leaf lex_node xs, \<not> sum.isl x]"
+
+paragraph \<open>Interlude: handling literal surrogates\<close>
+
+text \<open>
+JSON uses surrogate pairs like \<open>"\uD83D\uDE00"\<close>,
+in this case to encode the grinning emoji \<open>U+1F600\<close>.
+The lexer so far encodes this as the \<^emph>\<open>literal surrogate\<close> 6-byte sequence \<open>ED A0 BD ED B8 80\<close>.
+This is invalid UTF-8 and should be encoded as \<open>F0 9F 98 80\<close> instead.
+We therefore repair these intermediate literal surrogates.
+
+Note that the input to the lexer is assumed to be valid UTF-8,
+thus containing no literal surrogates.
+\<close>
+
+\<comment> \<open>Check if 3 bytes represent a High Surrogate (0xED 0xA0 0x80 - 0xED 0xAF 0xBF)\<close>
+definition is_high_byte_seq :: "char \<Rightarrow> char \<Rightarrow> char \<Rightarrow> bool" where
+  "is_high_byte_seq b1 b2 b3 \<longleftrightarrow>
+    (nat_of_char b1 = 0xED \<and>
+     nat_of_char b2 \<ge> 0xA0 \<and> nat_of_char b2 \<le> 0xAF \<and>
+     nat_of_char b3 \<ge> 0x80 \<and> nat_of_char b3 \<le> 0xBF)"
+
+\<comment> \<open>Check if 3 bytes represent a Low Surrogate (0xED 0xB0 0x80 - 0xED 0xBF 0xBF)\<close>
+definition is_low_byte_seq :: "char \<Rightarrow> char \<Rightarrow> char \<Rightarrow> bool" where
+  "is_low_byte_seq b1 b2 b3 \<longleftrightarrow>
+    (nat_of_char b1 = 0xED \<and>
+     nat_of_char b2 \<ge> 0xB0 \<and> nat_of_char b2 \<le> 0xBF \<and>
+     nat_of_char b3 \<ge> 0x80 \<and> nat_of_char b3 \<le> 0xBF)"
+
+definition extract_10_bits :: "char \<Rightarrow> char \<Rightarrow> nat" where
+  "extract_10_bits b2 b3 = ((nat_of_char b2 mod 16) * 64 + (nat_of_char b3 mod 64))"
+
+definition encode_utf8_4 :: "nat \<Rightarrow> nat \<Rightarrow> char list" where
+  "encode_utf8_4 hi_bits lo_bits = (
+     let u = (hi_bits * 1024) + lo_bits + 65536 in
+     [char_of (240 + (u div 262144)),             \<comment> \<open>0xF0 + bits\<close>
+      char_of (128 + ((u div 4096) mod 64)),      \<comment> \<open>0x80 + bits\<close>
+      char_of (128 + ((u div 64) mod 64)),        \<comment> \<open>0x80 + bits\<close>
+      char_of (128 + (u mod 64))])"               \<comment> \<open>0x80 + bits\<close>
+
+fun repair_bytes :: "string \<Rightarrow> string option" where
+  "repair_bytes (h1 # h2 # h3 # l1 # l2 # l3 # cs) = (
+     if is_high_byte_seq h1 h2 h3 \<and> is_low_byte_seq l1 l2 l3 then
+       (case repair_bytes cs of
+          Some rest \<Rightarrow> Some (encode_utf8_4 (extract_10_bits h2 h3) (extract_10_bits l2 l3) @ rest)
+        | None \<Rightarrow> None)
+     else if is_high_byte_seq h1 h2 h3 then None \<comment> \<open>Lone High\<close>
+     else (case repair_bytes (h2 # h3 # l1 # l2 # l3 # cs) of
+             Some rest \<Rightarrow> Some (h1 # rest) | None \<Rightarrow> None)
+  )" |
+  "repair_bytes (b1 # b2 # b3 # cs) = (
+     if is_high_byte_seq b1 b2 b3 \<or> is_low_byte_seq b1 b2 b3 then None
+     else (case repair_bytes (b2 # b3 # cs) of Some rest \<Rightarrow> Some (b1 # rest) | None \<Rightarrow> None)
+  )" |
+  "repair_bytes (c # cs) = (case repair_bytes cs of Some rest \<Rightarrow> Some (c # rest) | None \<Rightarrow> None)" |
+  "repair_bytes [] = Some []"
+
+\<comment> \<open>Repairing the surrogate for the grinning emoji\<close>
+lemma "repair_bytes [CHR 0xED, CHR 0xA0, CHR 0xBD, CHR 0xED, CHR 0xB8, CHR 0x80]
+  = Some [CHR 0xF0, CHR 0x9F, CHR 0x98, CHR 0x80]"
+  by eval
+
+\<comment> \<open>Lone surrogates are rejected\<close>
+lemma
+  "repair_bytes [CHR 0xED, CHR 0xA0, CHR 0xBD] = None"
+  by eval
+
+\<comment> \<open>ASCII strings are unchanged\<close>
+lemma
+  "repair_bytes ''test'' = Some ''test''"
+  by eval
+
+fun map_surrogates_lex where
+  "map_surrogates_lex (LStr x) = map_option LStr (repair_bytes x)"
+| "map_surrogates_lex x = Some x"
+
+definition map_surrogates where
+  "map_surrogates ps = those (
+    map (\<lambda>(k, v). map_option (Product_Type.Pair k) (map_surrogates_lex v)) ps)"
+
+subsection \<open>Putting everything together\<close>
+
+definition lex_it where
+  "lex_it x \<equiv>
+  let
+    chrs = mk_chrs x;
+    lex_result = parse lex_pt (NT (start jsonLex)) chrs
+  in
+    case lex_result of
+      RESULT t r \<Rightarrow>
+      if r = [] then
+        case map_surrogates (lex_tree_to_lex_list t) of
+          None \<Rightarrow> Inl ''Lone surrogates not allowed''
+        | Some ps \<Rightarrow> Inr ps
+      else
+        Inl ''Remaining characters''
+    | REJECT e _ \<Rightarrow> Inl e"
+
+definition parse_it where
+  "parse_it x \<equiv>
+  let
+    result = parse pt (NT (start jsonGrammar)) x
+   in
+    case result of
+      RESULT t r \<Rightarrow>
+      if r = [] then
+        Inr (parse_tree_to_json t)
+      else
+        Inl ''Remaining tokens''
+    | REJECT e _ \<Rightarrow> Inl e"
+
+definition
+  "json_from_string x \<equiv>
+  case lex_it x of
+    Inr t \<Rightarrow> (case parse_it t of
+      Inr x \<Rightarrow> Inr x
+    | Inl e \<Rightarrow> Inl (''Parsing error: '' @ e))
+  | Inl e \<Rightarrow> Inl (''Lexing error: '' @ e)"
+
+subsection \<open>Examples\<close>
+
+definition ex1 :: string where
+  "ex1 \<equiv> ''
+  {
+  \"items\": [
+    {
+    \"id\":           65,
+    \"description\":  \"Title\",
+    \"visible\":      false},
+    {
+    \"id\":           42,
+    \"visible\":      true}
+  ]
+}''
+"
+
+definition
+  "json_int i = JSON.Num (JsonNumber (i < 0) (nat (abs i)) None False None)"
+
+lemma "json_from_string ex1 = Inr (
+  Object
+  [(''items'',
+    Array
+     [Object
+       [(''id'', json_int 65),
+        (''description'', String ''Title''),
+        (''visible'', Boolean False)],
+      Object
+       [(''id'', json_int 42), (''visible'', Boolean True)]])])"
+  by eval
+
+lemma "json_from_string ''{\"test\": null, \"test\": 67}''
+  = Inr (Object [(''test'', JSON.Nil), (''test'', json_int 67)])"
+  by eval
+
+lemma "json_from_string ''{\"test\": null, \"test\": [67], \"a\": false}''
+  = Inr (Object [(''test'', JSON.Nil), (''test'', Array [json_int 67]), (''a'', Boolean False)])"
+  by eval
+
+lemma "json_from_string ''\",+-0][{}\"'' = Inr (String '',+-0][{}'')"
+  by eval
+
+lemma "json_from_string ''\"\"'' = Inr (String [])"
+  by eval
+
+lemma "json_from_string ''\"a\"'' = Inr (String ''a'')"
+  by eval
+
+text \<open>Escape characters\<close>
+lemma "json_from_string (
+    CHR ''\"'' # CHR 0x5C # ''\"cb'' @ CHR 0x5C # ''n'' @ CHR 0x5C # CHR 0x5C
+  # CHR 0x5C # ''b'' @ CHR 0x5C # ''r'' @ CHR 0x5C # ''t\"'')
+  = Inr (String
+      [CHR ''\"'', CHR ''c'', CHR ''b'', CHR ''\<newline>'', CHR 0x5C, CHR 8, CHR 13, CHR 9])"
+  by eval
+
+lemma "json_from_string ''[-0]'' = Inr (JSON.Array [JSON.Num (JsonNumber True 0 None False None)])"
+  by eval
+
+lemma "json_from_string ''[1,2, 123,1, 0,\<newline>-1,-12]''
+  = Inr (Array (map json_int [1, 2, 123, 1, 0, -1, - 12]))"
+  by eval
+
+lemma "json_from_string ''[1.0,1.021,0.2]''
+  = Inr (Array
+       [Num (JsonNumber False 1 (Some ''0'')  False None),
+        Num (JsonNumber False 1 (Some ''021'') False None),
+        Num (JsonNumber False 0 (Some ''2'')  False None)])"
+  by eval
+
+lemma
+  "json_from_string ''[12E-2, 1e2, 33E+2 , 3.3E+2,-1.3e-23, 1.3E0, 1e-0, -0e+0000]''
+  = Inr (Array
+       [Num (JsonNumber False 12 (Some []) True (Some 2)),
+        Num (JsonNumber False 1 (Some []) False (Some 2)),
+        Num (JsonNumber False 33 (Some []) False (Some 2)),
+        Num (JsonNumber False 3 (Some ''3'') False (Some 2)),
+        Num (JsonNumber True 1 (Some ''3'') True (Some 23)),
+        Num (JsonNumber False 1 (Some ''3'') False (Some 0)),
+        Num (JsonNumber False 1 (Some []) True (Some 0)),
+        Num (JsonNumber True 0 (Some []) False (Some 0))])"
+  by eval
+
+lemma "json_from_string ''\"a\",'' = Inl ''Parsing error: Remaining tokens''"
+  by eval
+
+lemma "json_from_string ''00'' = Inl ''Lexing error: lookup failure''"
+  by eval
+
+lemma "json_from_string (''\"a'' @ CHR 0x5C # ''ud800\"'')
+  = Inl ''Lexing error: Lone surrogates not allowed''"
+  by eval
+
+\<comment> \<open>\<open>U+1F600\<close>\<close>
+lemma "json_from_string (''\"'' @ CHR 0x5C # ''uD83D'' @ CHR 0x5C # ''uDE00\"'')
+  = Inr (String [CHR 0xF0, CHR 0x9F, CHR 0x98, CHR 0x80])"
+  by eval
+
+\<comment> \<open>\<open>\<lambda>\<close>\<close>
+lemma "json_from_string (''\"'' @ CHR 0x5C # ''u03BB\"'')
+  = Inr (String [CHR 0xCE, CHR 0xBB])"
+  by eval
+
+\<comment> \<open>\<open>"a "\<close>\<close>
+lemma "json_from_string (''\"a'' @ CHR 0x5C # ''u0020\"'') = Inr (String ''a '')"
+  by eval
+
+subsection \<open>Printing JSON\<close>
+
+definition
+  "pad m s = replicate m CHR '' '' @ s"
+
+definition app where "app a b \<equiv> b a"
+
+notation (input) app (infixl "|>" 59)
+
+fun intersperse :: "'a \<Rightarrow> 'a list \<Rightarrow> 'a list" where
+  "intersperse sep (x # y # xs) = x # sep # intersperse sep (y # xs)"
+| "intersperse _ xs = xs"
+
+fun hex_digit :: "nat \<Rightarrow> char" where
+  "hex_digit n =
+     (if n < 10 then char_of (48 + n) else char_of (55 + n))"
+
+fun hex2 :: "nat \<Rightarrow> string" where
+  "hex2 n =
+     [hex_digit (n div 16), hex_digit (n mod 16)]"
+
+fun escape_char :: "char \<Rightarrow> string" where
+  "escape_char c =
+     (if c = CHR 0x22 then
+        [CHR 0x5C, CHR 0x22]      \<comment> \<open>\"\<close>
+      else if c = CHR 0x5C then
+        [CHR 0x5C, CHR 0x5C]      \<comment> \<open>\\\<close>
+      else if c = CHR 0x08 then
+        [CHR 0x5C, CHR 0x62]      \<comment> \<open>\\b\<close>
+      else if c = CHR 0x0C then
+        [CHR 0x5C, CHR 0x66]      \<comment> \<open>\\f\<close>
+      else if c = CHR 0x0A then
+        [CHR 0x5C, CHR 0x6E]      \<comment> \<open>\\n\<close>
+      else if c = CHR 0x0D then
+        [CHR 0x5C, CHR 0x72]      \<comment> \<open>\\r\<close>
+      else if c = CHR 0x09 then
+        [CHR 0x5C, CHR 0x74]      \<comment> \<open>\\t\<close>
+      else if nat_of_char c < 32 then
+        [CHR 0x5C, CHR 0x75, CHR 0x30, CHR 0x30]
+          @ hex2 (nat_of_char c)  \<comment> \<open>\\u00XX\<close>
+      else
+        [c])"
+
+fun escape_string :: "string \<Rightarrow> string" where
+  "escape_string [] = []"
+| "escape_string (c # cs) = escape_char c @ escape_string cs"
+
+fun shows_json_number where
+  "shows_json_number (JsonNumber s n None se None) = (if s then ''-'' else '''') @ show n"
+| "shows_json_number (JsonNumber s n (Some f) se None)
+  = (if s then ''-'' else '''') @ show n @ ''.'' @ f"
+| "shows_json_number (JsonNumber s n None se (Some e))
+  = (if s then ''-'' else '''') @ show n @ ''E'' @ (if se then ''-'' else '''') @ show e"
+| "shows_json_number (JsonNumber s n (Some f) se (Some e))
+  = (if s then ''-'' else '''') @ show n @ ''.'' @ f @ ''E'' @ (if se then ''-'' else '''') @ show e"
+
+fun shows_json :: "nat \<Rightarrow> JSON \<Rightarrow> string" where
+  "shows_json n (Num m) = shows_json_number m |> pad n"
+| "shows_json n (Boolean b) = (if b then ''true'' else ''false'') |> pad n"
+| "shows_json n Nil = ''null'' |> pad n"
+| "shows_json n (String s) = pad n (''\"'' @ escape_string s @ ''\"'')"
+| "shows_json n (JSON.Array xs) = (
+  if xs = [] then
+    pad n ''[]''
+  else
+    pad n ''[\<newline>''
+    @ concat (map (shows_json (n + 2)) xs |> intersperse '',\<newline>'')
+    @ ''\<newline>''
+    @ pad n '']''
+  )"
+| "shows_json n (JSON.Object xs) = (
+  if xs = [] then
+    pad n ''{}''
+  else
+    pad n ''{\<newline>''
+    @ concat (
+      map (\<lambda>(k, v).
+        pad (n + 2) (''\"'' @ escape_string k @ ''\"'') @ '':\<newline>'' @ shows_json (n + 4) v) xs
+      |> intersperse '',\<newline>''
+    )
+    @ ''\<newline>''
+    @ pad n ''}''
+  )"
+
+instantiation JSON :: "show"
+begin
+
+definition "shows_prec p (x :: JSON) rest = shows_json 0 x @ rest" for p
+
+definition "shows_list jsons s =
+  map (shows_json 0) jsons |> intersperse '', '' |> (\<lambda>xs. ''['' @ concat xs @ '']'' @ s)"
+instance
+  by standard (simp_all add: shows_prec_JSON_def shows_list_JSON_def show_law_simps app_def)
+
+end
+
+no_notation (input) app (infixl "|>" 59)
+
+paragraph \<open>Testing round-trips\<close>
+
+lemma
+  "json_from_string (show (sum.projr (json_from_string ex1))) = json_from_string ex1"
+  by eval
+
+definition
+  "rm_ws s = [c . c \<leftarrow> s, \<not> is_ws c]"
+
+\<comment> \<open>This property will not generally hold in the presence of escaped unicode characters.\<close>
+lemma "rm_ws (show (sum.projr (json_from_string ex1))) = rm_ws ex1"
+  by eval
+
+definition ex_rcf8259 where
+  "ex_rcf8259 \<equiv>
+''{
+  \"Image\": {
+      \"Width\":  800,
+      \"Height\": 600,
+      \"Title\":  \"View from 15th Floor\",
+      \"Thumbnail\": {
+          \"Url\":    \"http://www.example.com/image/481989943\",
+          \"Height\": 125,
+          \"Width\":  100
+      },
+      \"Animated\" : false,
+      \"IDs\": [116, 943, 234, 38793]
+    }
+}''"
+
+lemma
+  "json_from_string (show (sum.projr (json_from_string ex_rcf8259))) = json_from_string ex_rcf8259"
+  by eval
+
+lemma "rm_ws (show (sum.projr (json_from_string ex_rcf8259))) = rm_ws ex_rcf8259"
+  by eval
 
 end
